thys/Pi_Calculus/Pi_Transition_Late.thy
@@ -20,126 +20,29 @@ binder_inductive trans
         | ((rule exI[of _ "\<sigma> _"] exI)+, (rule conjI)?, rule refl)
         | (rule exI[of _ "map_action \<sigma> _"] exI[of _ "rrename \<sigma> _"])
         | ((rule exI[of _ "\<sigma> _"])+; auto))+
-
-  subgoal premises prems for R B x1 x2
-  proof -
-    define G where "G \<equiv> \<lambda>B p x1 x2.
-                (\<exists>a x P. B = {x} \<and> x1 = Inp a x P \<and> x2 = Binp a x P) \<or>
-                (\<exists>P a x P' Q y Q'. B = {x} \<and> x1 = P \<parallel> Q \<and> x2 = Tau (P'[y/x] \<parallel> Q') \<and> p P (Binp a x P') \<and> p Q (Fout a y Q')) \<or>
-                (\<exists>P a x P' Q Q'. B = {x} \<and> x1 = P \<parallel> Q \<and> x2 = Tau (Res x (P' \<parallel> Q')) \<and> p P (Binp a x P') \<and> p Q (Bout a x Q')) \<or>
-                (\<exists>P a x P'. B = {x} \<and> x1 = Res x P \<and> x2 = Bout a x P' \<and> p P (Fout a x P') \<and> a \<noteq> x) \<or>
-                (\<exists>P \<alpha> P' x. B = insert x (bvars \<alpha>) \<and> x1 = Res x P \<and> x2 = Cmt \<alpha> (Res x P') \<and> p P (Cmt \<alpha> P') \<and> fra \<alpha> \<and> x \<notin> ns \<alpha>) \<or>
-                (\<exists>P a x P' y. B = {x, y} \<and> x1 = Res y P \<and> x2 = Bout a x (Res y P') \<and> p P (Bout a x P') \<and> y \<notin> {a, x} \<and> x \<notin> FFVars P \<union> {a}) \<or>
-                (\<exists>P \<alpha> P' Q. B = bvars \<alpha> \<and> x1 = P \<parallel> Q \<and> x2 = Cmt \<alpha> (P' \<parallel> Q) \<and> p P (Cmt \<alpha> P') \<and> bvars \<alpha> \<inter> (FFVars P \<union> FFVars Q) = {})"
-    { assume assms: "(\<forall>\<sigma> x1 x2. isPerm \<sigma> \<and> R x1 x2 \<longrightarrow> R (rrename \<sigma> x1) (rrename_commit \<sigma> x2))"
-      have "G B R x1 x2 \<Longrightarrow> \<exists>C. C \<inter> Tsupp x1 x2 = {} \<and> G C R x1 x2"
-        unfolding G_def
-          isPerm_def conj_assoc[symmetric]
-        unfolding ex_push_inwards conj_disj_distribL ex_disj_distrib ex_simps(1,2)[symmetric]
-          ex_comm[where P = P for P :: "_ set \<Rightarrow> _ \<Rightarrow> _"]
-        apply (elim disj_forward exE; simp; tactic \<open>REPEAT_DETERM_N 2 (gen_fresh @{context} [] [] [@{term x1}, @{term x2}])\<close>; clarsimp)
-              apply ((((rule exI conjI)+)?, (assumption | rule Inp_refresh Res_refresh usub_refresh arg_cong2[where f=Cmt, OF refl])
-               | (erule (1) R_forw_subst[of R, OF _ assms[simplified, rule_format, OF conjI[OF isPerm_swap]]]; simp?)
-               | (auto simp only: fst_conv snd_conv term.set FFVars_commit_simps FFVars_commit_Cmt act_var_simps))+)[2]
-        apply (metis Inp_refresh)
-        subgoal for P1 a x P1' P2 y P2' z1 z2
-          apply (rule exI[of _ a])
-          apply (rule exI[of _ z1])
-          apply (rule conjI) apply assumption
-          apply safe
-          apply simp
-          apply (rule exI[of _ "swap P1' x z1"])
-          apply (rule exI[of _ y])
-          apply (rule conjI)
-          apply (metis UnI1 insert_Diff insert_iff usub_refresh)
-          apply (rule conjI)
-          apply (metis Binp_inj UnI1 insert_Diff insert_iff)
-          apply assumption
-          done
-
-        subgoal for P a x P' Q y Q' xa xb
-        proof -
-          assume a1: "R P (Binp a x P')"
-          assume a2: "R Q (Fout a y Q')"
-          assume a3: "xb \<notin> FFVars P"
-          assume a4: "xb \<notin> FFVars Q"
-          assume a5: "xb \<notin> (if False then FFVars P' - {x} \<union> {y} else FFVars P')"
-          assume a6: "xb \<notin> FFVars Q'"
-          have "\<forall>v va. Binp v va P' = Binp v xb (swap P' va xb)"
-            using a5 Binp_inj by presburger
-          then show ?thesis
-            using a6 a5 a4 a3 a2 a1 by (metis (no_types) usub_refresh)
-        qed
-
-        subgoal for P1 a x P1' P2 P2' z1 z2
-          apply (rule exI[of _ a])
-          apply (rule exI[of _ z1])
-          apply (rule conjI) apply assumption
-          apply safe
-          apply (rule exI[of _ "swap P1' x z1"])
-          apply (rule exI[of _ "swap P2' x z1"])
-          apply (intro conjI)
-            apply (simp add: Res_refresh[of z1 "Par P1' P2'" x])
-           apply (metis Binp_inj)
-          by (metis Bout_inj)
-
-           apply ((((rule exI conjI)+)?, (assumption | rule Inp_refresh Res_refresh usub_refresh arg_cong2[where f=Cmt, OF refl])
-              | (erule (1) R_forw_subst[of R, OF _ assms[simplified, rule_format, OF conjI[OF isPerm_swap]]]; simp?)
-              | (auto simp only: fst_conv snd_conv term.set FFVars_commit_simps FFVars_commit_Cmt act_var_simps))+) [1]
-        apply simp
-        apply (smt (verit) Diff_disjoint Diff_empty FFVars_commit_Cmt UnE action.simps(65) action.simps(66) action.simps(69) bns.simps(1) bns.simps(2) empty_bvars_vars_fvars inf_bot_left insert_disjoint(2) insert_not_empty ns.elims term.set(8))
-
-        subgoal for P a x P' y z1 z2
-          apply (rule exI[of _ "swap P y z1"])
-          apply (rule exI[of _ a])
-          apply (rule exI[of _ z2])
-          apply (rule conjI) apply simp
-          apply (rule exI[of _ "swap (swap P' x z2) y z1"])
-          apply (rule exI[of _ z1])
-          apply (rule conjI) apply simp
-          apply clarsimp
-          apply ((((rule exI conjI)+)?, (assumption | rule Inp_refresh Res_refresh usub_refresh arg_cong2[where f=Cmt, OF refl] refl)))
-           apply auto[]
-          apply (rule conjI[OF sym])
-           apply ((((rule exI conjI)+)?, (assumption | rule Inp_refresh Res_refresh usub_refresh arg_cong2[where f=Cmt, OF refl] refl)))
-          apply simp
-           apply (smt (verit, best) image_iff sw_diff sw_eqR)
-          apply (rule conjI)
-           apply (erule (1) R_forw_subst[of R, OF _ assms[simplified, rule_format, OF conjI[OF isPerm_swap]]]; simp?)
-           apply (rule conjI)
-            apply (smt (verit, best) image_iff sw_diff sw_eqR)
-           apply (simp add: swap_commute term.rrename_comps[where w="swap P' y z1"] supp_comp_bound[OF _ _ infinite_UNIV]
-              term.rrename_cong_ids[symmetric])
-          apply (smt (verit, best) image_iff sw_diff sw_eqR)
-          done
-
-        subgoal for P1 act P1' P2 z1 z2
-          using bvars_act_bout[of act]
-          apply (elim disjE exE)
-            apply (rule exI[of _ act])
-            apply auto
-          subgoal for a b
-            apply (intro exI[of _ "bout a z1"] conjI)
-              apply simp
-             apply simp
-            apply (intro exI[of _ "swap P1' b z1"] conjI)
-              apply simp
-             apply simp
-             apply (metis Bout_inj)
-            apply simp
-            done
-
-          subgoal for a b
-            apply (intro exI[of _ "binp a z1"] conjI)
-             apply simp+
-             apply (metis Binp_inj)
-            done
-          done
-        done
-    } note 1 = this
-    then show ?thesis using prems(2,3) unfolding G_def isPerm_def by simp
-  qed
-done
+  subgoal premises prems for R B P Q
+    by (tactic \<open>refreshability_tac true
+      [@{term "FFVars :: trm \<Rightarrow> var set"}, @{term "FFVars_commit :: cmt \<Rightarrow> var set"}]
+      [@{term "rrename :: (var \<Rightarrow> var) \<Rightarrow> trm \<Rightarrow> trm"}, @{term "(\<lambda>f x. f x) :: (var \<Rightarrow> var) \<Rightarrow> var \<Rightarrow> var"},
+       @{term "rrename_bound_action :: (var \<Rightarrow> var) \<Rightarrow> var action \<Rightarrow> var action"}]
+      [SOME [NONE, SOME 1, SOME 0],
+       SOME [NONE, NONE, SOME 1, SOME 0, NONE, NONE, NONE],
+       SOME [NONE, NONE, SOME 1, SOME 0, NONE, SOME 0],
+       SOME [SOME 0, NONE, SOME 1, SOME 0],
+       SOME [SOME 0, NONE, SOME 0, SOME 1],
+       SOME [SOME 0, NONE, SOME 1, SOME 0, SOME 1],
+       SOME [NONE, SOME 2, SOME 0, SOME 0]]
+      @{thm prems(3)} @{thm prems(2)} @{thms }
+      @{thms emp_bound singl_bound insert_bound card_of_minus_bound term.Un_bound term.card_of_FFVars_bounds commit_internal.card_of_FFVars_bounds infinite_UNIV bns_bound}
+      @{thms Res_inject Inp_inject Bout_inject FFVars_commit_Cmt ns_alt vars_alt Int_Un_distrib}
+      @{thms Inp_eq_usub rrename_cong term.rrename_cong_ids term.rrename_cong_ids[symmetric] arg_cong2[where f=Cmt, OF _ refl] arg_cong2[where f=Cmt, OF refl]
+          action.map_ident_strong cong[OF arg_cong2[OF _ refl] refl, of _ _ Bout] Cmt_rrename_bound_action Cmt_rrename_bound_action_Par}
+      @{thms cong[OF cong[OF refl[of R] refl], THEN iffD1, rotated -1, of _ _ "Bout _ _ _"] id_onD id_on_antimono
+             cong[OF cong[OF refl[of R] refl], THEN iffD1, rotated -1, of _ _ "Fout _ _ _"]
+             cong[OF cong[OF refl[of R] refl], THEN iffD1, rotated -1, of _ _ "Cmt _ _"]
+             cong[OF cong[OF refl[of R] refl], THEN iffD1, rotated -1, of _ _ "Binp _ _ _"]
+             cong[OF cong[OF refl[of R] term.rrename_cong_ids], THEN iffD1, rotated -1, of _ _ _ "Finp _ _ _"]} @{context}\<close>)
+  done
 print_theorems
 
 end
